Surface/Global.lean
@@ -217,3 +217,10 @@ theorem Surface.Global.lookup_type_unique :
   t = t' := by
 intro h1 h2
 all_goals (rw[h1] at h2; injection h2)
+
+theorem Surface.Global.lookup_kind_unique :
+  lookup_kind x G = some t ->
+  lookup_kind x G = some t' ->
+  t = t' := by
+intro h1 h2
+all_goals (rw[h1] at h2; injection h2)
