Translation/Global/Lemmas.lean
@@ -4,31 +4,127 @@ import Core.Global
 import Surface.Typing
 import Core.Typing
 
+import Translation.Ty.Lemmas
+import Translation.Term.Lemmas
+
 theorem Translation.Ty.valid_ctor_ty_sound {G : Core.GlobalEnv} :
-  Core.is_valid_ctor_ty G T == some () -> ∃ x, Core.ValidCtor x T := by
+  Core.is_valid_ctor_ty G T == some x -> Core.ValidCtor x T := by
 intro h
 fun_induction Core.is_valid_ctor_ty <;> simp at *
-case _ ih => replace ih := ih h; rcases ih with ⟨x, ih⟩; exists x; apply Core.ValidCtor.all ih
-case _ ih => replace ih := ih h; rcases ih with ⟨x, ih⟩; exists x; apply Core.ValidCtor.arrow ih
+case _ ih => replace ih := ih h; apply Core.ValidCtor.all ih
+case _ ih => replace ih := ih h; apply Core.ValidCtor.arrow ih
 case _ =>
-  rw[Option.bind_eq_some_iff] at h; rcases h with ⟨tnf, h1, h2⟩; exists tnf.1; simp at h2;
+  rw[Option.bind_eq_some_iff] at h; rcases h with ⟨tnf, h1, h2⟩;
+  simp at h2; rcases h2 with ⟨h2, e⟩; subst x
   apply Core.ValidCtor.base; apply h1
+
+theorem Translation.Ty.ValidCtor :
+  Surface.ValidCtor x T -> Core.ValidCtor x ⟦T⟧ := by
+intro h; induction h <;> simp at *
+case base h =>
+  replace lem := Translation.Ty.Spine h rfl
+  rcases lem with ⟨_, lem⟩
+  constructor; assumption
+case all ih => apply Core.ValidCtor.all ih
+case arrow ih => apply Core.ValidCtor.arrow ih
+
+theorem Translation.Ty.valid_ctor_ty_complete {G : Core.GlobalEnv}:
+  Core.is_data G x ->
+  Core.ValidCtor x T -> Core.is_valid_ctor_ty G T == some x := by
+intro h1 h
+induction T using Core.is_valid_ctor_ty.induct generalizing G x <;> simp [Core.is_valid_ctor_ty] at *
+case _ ih =>
+  cases h
+  case _ h => simp [Core.Ty.spine] at h
+  case _ h => apply ih h1 h
+case _ ih =>
+  cases h
+  case _ h => simp [Core.Ty.spine] at h
+  case _ h => apply ih h1 h
+case _ =>
+  rw[Option.bind_eq_some_iff];
+  cases h
+  case base sp tnf =>
+    exists (x, sp)
+    apply And.intro
+    apply tnf
+    simp; assumption
+  case _ h => simp [Core.Ty.spine]; sorry
+  case _ => simp [Core.Ty.spine]; sorry
+
+-- induction h <;> simp [Core.is_valid_ctor_ty] at *
+-- case all ih => assumption
+-- case arrow => assumption
+-- case base => sorry
+
+theorem Translation.Global.empty_data_wkn {G : Surface.GlobalEnv} {G' : Core.GlobalEnv} (x : String) (K : Surface.Kind) :
+  G.translate = some G' ->
+  Surface.GlobalEnv.translate (.data x K Vect.nil :: G) = some (.data 0 x ⟦K⟧ Vect.nil :: G') := by
+intro h; simp [Surface.GlobalEnv.translate]
+rw[Option.bind_eq_some_iff]; exists G'
+
+theorem Surface.GlobalEnvWf.empty_data_wkn x K : ⊢s G -> lookup x G = none -> ⊢s (Surface.Global.data x K Vect.nil :: G) := by
+ intro wf lk; apply ListGlobalWf.cons
+ · apply GlobalWf.data <;> try simp at *
+   apply Vect.nil
+   apply lk
+ · assumption
 
 
 theorem Translation.GlobalWf.sound {G : Surface.GlobalEnv} {g : Surface.Global}:
   ⊢s G ->
   Surface.GlobalWf G g ->
   G.translate = some G' ->
+  (∀ x, Surface.lookup x G = none -> Core.lookup x G' = none) ->
   ⊢ G' ->
  ∃ g',
     g.translate G' = some g'  ∧
     Core.GlobalWf G' g' := by
-intro wf h1 h2 wfc; induction g <;> simp at *
+intro wf h1 h2 h3 wfc; induction g <;> simp at *
 cases h1
-case _ n x K ctors cns cnsu lk cnsdef ctor_trans =>
-let ctors' : Vect n (String × Core.Ty) := sorry --Vect.seq
+case _ n x K ctors cns lk cnsdef ctor_trans =>
+let ctors' : Vect n (String × Core.Ty) := (λ x => (x.fst , x.snd.translate)) <$> ctors
 exists Core.Global.data n x ⟦K⟧ ctors'
-sorry
+rw[Option.bind_eq_some_iff];
+apply And.intro
+· exists ctors';
+  apply And.intro
+  · simp [Surface.Ty.translate_ctors]
+
+    unfold Vect.seq;
+    generalize zdef : Vect.seq_lemma (fun n =>
+        (Core.is_valid_ctor_ty (Core.Global.data 0 x ⟦K⟧ Vect.nil :: G') ⟦(ctors n).snd⟧).bind fun __discr =>
+          some ((ctors n).fst, ⟦(ctors n).snd⟧)) = z at *
+    cases z <;> simp at *
+    case inr v => funext; case _ i =>   unfold ctors'; simp
+    case inl v =>
+      rcases v with ⟨j, v⟩
+      have lem := Option.not_isSome_iff_eq_none.1 v
+      replace lem := Option.bind_eq_none'.1 lem ((ctors j).fst , ⟦(ctors j).snd⟧) x
+      replace ctor_trans := ctor_trans j (ctors j).fst (ctors j).snd rfl
+      rcases ctor_trans with ⟨k1, k2, k3, k4⟩
+      have k2' := Translation.Ty.ValidCtor k2
+      sorry
+
+  · simp
+· apply Core.GlobalWf.data
+  · intro i y T e;
+    replace ctor_trans := ctor_trans i (ctors i).fst (ctors i).snd rfl;
+    rcases ctor_trans with ⟨k1, k2, k3, k4⟩
+    simp [ctors'] at e; rcases e with ⟨e1, e2⟩; subst y; subst T
+    apply And.intro
+    · have lemG := Translation.Global.empty_data_wkn x K h2
+      have wfG := Surface.GlobalEnvWf.empty_data_wkn x K wf lk
+      have lem := Translation.Ty.sound wfG (G := .data x K Vect.nil :: G) ⟨k1,lemG, rfl⟩
+      rcases lem with ⟨K', T', e1, e2, e3⟩;
+      simp at e1; subst e1; subst e2; simp [Surface.KindEnv.translate] at e3; apply e3
+    · apply And.intro
+      · apply Translation.Ty.ValidCtor k2
+      · apply And.intro; assumption;
+        apply h3; apply k4
+  · assumption
+  · apply h3 _ lk
+
 
 theorem Translation.ListGlobalWf.sound_isSome :
   ⊢s G ->
@@ -41,7 +137,9 @@ theorem Translation.ListGlobalWf.wf_preserved :
   G.translate = some G' ->
   ⊢ G'
 := by
-  sorry
+  intro wf h1; induction wf generalizing G' <;> simp at *
+  case nil => sorry
+  case cons => sorry
 
 theorem Translation.ListGlobalWf.sound2 {G : Surface.GlobalEnv} :
   ⊢s G ->
