Translation/Ty/Lemmas.lean
@@ -32,7 +32,17 @@ theorem Translation.GlobalEnv.lookup_kind_sound :
   Surface.lookup_kind G x = some K ->
   Core.lookup_kind G' x = some K'  := by
 intro h1 h2
-sorry
+fun_induction Surface.GlobalEnv.translate generalizing G' <;> simp [Surface.lookup_kind, Surface.lookup] at h2
+case _ g gs ih =>
+  cases g <;> simp at *
+  case _ y _ _ =>
+  generalize zdef : (x == y) = z at *
+  cases z <;> simp at *
+  · sorry
+  · subst y; simp [Surface.Entry.kind] at h2; sorry
+
+
+
 
 
 theorem Translation.Ty.sound :
